\documentclass[a4paper,12pt]{report}
\usepackage[utf8]{inputenc}
\usepackage[T1]{fontenc}
\usepackage[french]{babel}
\usepackage{amsmath, amssymb}
\newcommand{\abs}[1]{\lvert#1\rvert}%la valeur absolue
\begin{document}
\begin{enumerate}
\item Développons et réduisons $(x-1)^3$.

$\begin{aligned}
(x-1)^3 &= (x-1)(x-1)^2\\
			&=(x-1)(x^2-2x+1)\\
			&=x^3-2x^2+x-x^2+2x-1\\
			&=x^3-3x^2+3x-1
\end{aligned}$

\item Résoudre l'équation
$x^3-3x^2+3x-1=0$ dans
 $\mathbb{R}$.

\[\begin{aligned}
x^3-3x^2+3x-1=0 &\iff (x-1)^3=0\\
							  &\iff x-1=0\\
							  &\iff x=1
\end{aligned}\]

L'ensemble des solutions de
l'équation est $\{1\}$.
\end{enumerate}
\end{document}
